Builds. Examples fixing.

examples/Nimp.v
@@ -1,4 +1,5 @@
 (* A nondeterministic Imp *)
+From Coinduction Require Import all. 
 
 From Stdlib Require Import
      Relations.
@@ -29,24 +30,24 @@ Example choose_loop : com := choose (loop skip) skip.
 (* Unlabeled small-step *)
 Module Unlabeled.
 
-Reserved Infix "-->" (at level 80, no associativity).
+Reserved Infix "--->" (at level 80, no associativity).
 
 Inductive step : relation com :=
 | step_loop_stop c :
-    loop c --> skip
+    loop c ---> skip
 | step_loop_go c :
-    loop c --> (c ;; loop c)
+    loop c ---> (c ;; loop c)
 | step_choose_l c1 c2 :
-    choose c1 c2 --> c1
+    choose c1 c2 ---> c1
 | step_choose_r c1 c2 :
-    choose c1 c2 --> c2
+    choose c1 c2 ---> c2
 | step_seq_go c1 c1' c2 :
-    c1 --> c2 ->
-    (c1 ;; c2) --> (c1' ;; c2)
+    c1 ---> c2 ->
+    (c1 ;; c2) ---> (c1' ;; c2)
 | step_seq_next c2 :
-    (skip ;; c2) --> c2
+    (skip ;; c2) ---> c2
 
-where "x --> y" := (step x y).
+where "x ---> y" := (step x y).
 
 CoInductive infinite_steps (c : com) : Type :=
 | more c' : step c c' -> infinite_steps c' -> infinite_steps c.
@@ -65,30 +66,30 @@ End Unlabeled.
 
 Module Labeled.
 
-Reserved Notation "s --> t" (at level 80, no associativity).
-Reserved Notation "s ! b --> t" (at level 80, b at next level, no associativity).
-Reserved Notation "s ? b --> t" (at level 80, b at next level, no associativity).
+Reserved Notation "s ---> t" (at level 80, no associativity).
+Reserved Notation "s ! b ---> t" (at level 80, b at next level, no associativity).
+Reserved Notation "s ? b ---> t" (at level 80, b at next level, no associativity).
 
 Variant label := tau | bit (b : bool).
 
 Inductive step : label -> relation com :=
 | step_loop_stop c :
-    loop c ! true --> skip
+    loop c ! true ---> skip
 | step_loop_go c :
-    loop c ! false --> (c ;; loop c)
+    loop c ! false ---> (c ;; loop c)
 | step_choose_l c1 c2 :
-    choose c1 c2 ! true --> c1
+    choose c1 c2 ! true ---> c1
 | step_choose_r c1 c2 :
-    choose c1 c2 ! false --> c2
+    choose c1 c2 ! false ---> c2
 | step_seq_go b c1 c1' c2 :
-    c1 ? b --> c2 ->
-    (c1 ;; c2) ? b --> (c1' ;; c2)
+    c1 ? b ---> c2 ->
+    (c1 ;; c2) ? b ---> (c1' ;; c2)
 | step_seq_next c2 :
-    (skip ;; c2) --> c2
+    (skip ;; c2) ---> c2
 
-where "x --> y" := (step tau x y)
-and  "x ! b --> y" := (step (bit b) x y)
-and  "x ? b --> y" := (step b x y).
+where "x ---> y" := (step tau x y)
+and  "x ! b ---> y" := (step (bit b) x y)
+and  "x ? b ---> y" := (step b x y).
 
 CoInductive infinite_steps (c : com) : Type :=
 | more b c' : step b c c' -> infinite_steps c' -> infinite_steps c.
@@ -104,8 +105,6 @@ Proof.
 Qed.
 
 End Labeled.
-
-From Paco Require Import paco.
 
 Module Tree.
 
@@ -156,7 +155,6 @@ Qed.
 (* SAZ: the [~] notation for eutt wasn't working here. *)
 Lemma eval_one_loop : eval one_loop ≈ one_loop_tree.
 Proof.
-  einit. ecofix CIH. edrop.
   setoid_rewrite rec_as_interp.
   setoid_rewrite interp_bind.
   setoid_rewrite interp_vis.
@@ -165,6 +163,7 @@ Proof.
   setoid_rewrite bind_bind.
   setoid_rewrite bind_ret_l.
   setoid_rewrite bind_vis.
+  step. 
   evis. intros.
   setoid_rewrite bind_ret_l.
   destruct v.
@@ -173,7 +172,7 @@ Proof.
     setoid_rewrite interp_recursive_call.
     setoid_rewrite eval_skip.
     setoid_rewrite bind_ret_l.
-    eauto with paco.
+    eauto.
 Qed.
 
 End Tree.
