theories/Basics/Utils.v
@@ -3,8 +3,6 @@
 From Coinduction Require Import all.
 Require Import Program.Tactics.
 
-From Paco Require Import paco.
-
 Ltac inv H := inversion H; clear H; subst; try easy.
 
 (* [inv], [rewrite_everywhere], [..._except] are general purpose *)
